backend/CSEproof.v
@@ -74,6 +74,17 @@ Proof.
 - econstructor; eauto. rewrite valnums_val_exten by assumption. auto.
 Qed.
 
+Lemma rhs_valid_exten:
+  forall r,
+  rhs_valid valu1 ge sp r ->
+  (forall v, In v (valnums_rhs r) -> Plt v upto) ->
+  rhs_valid valu2 ge sp r.
+Proof.
+  intros. inv H; simpl in *.
+- constructor.
+- econstructor; eauto. rewrite valnums_val_exten by assumption. auto.
+Qed.
+
 Lemma equation_holds_exten:
   forall e,
   equation_holds valu1 ge sp m e ->
@@ -82,7 +93,9 @@ Lemma equation_holds_exten:
 Proof.
   intros. destruct e. destruct H0. inv H.
 - constructor. rewrite AGREE by auto. apply rhs_eval_to_exten; auto.
+  apply rhs_valid_exten; auto.
 - econstructor. apply rhs_eval_to_exten; eauto. rewrite AGREE by auto. auto.
+  apply rhs_valid_exten; auto.
 Qed.
 
 Lemma numbering_holds_exten:
@@ -176,24 +189,26 @@ Qed.
 
 Lemma find_valnum_rhs_charact:
   forall rh v eqs,
-  find_valnum_rhs rh eqs = Some v -> In (Eq v true rh) eqs.
+    find_valnum_rhs rh eqs = Some v ->
+    exists rh', In (Eq v true rh') eqs /\ rhs_compat rh rh'.
 Proof.
   induction eqs; simpl; intros.
 - inv H.
-- destruct a. destruct (strict && eq_rhs rh r) eqn:T.
-  + InvBooleans. inv H. left; auto.
-  + right; eauto.
+- destruct a. destruct (strict && compat_rhs rh r) eqn:T.
+  + InvBooleans. inv H. exists r; auto using compat_rhs_sound.
+  + destruct IHeqs as (rh' & A & B); auto. exists rh'; auto.
 Qed.
 
 Lemma find_valnum_rhs'_charact:
   forall rh v eqs,
-  find_valnum_rhs' rh eqs = Some v -> exists strict, In (Eq v strict rh) eqs.
+    find_valnum_rhs' rh eqs = Some v ->
+    exists strict rh', In (Eq v strict rh') eqs /\ rhs_compat rh rh'.
 Proof.
   induction eqs; simpl; intros.
 - inv H.
-- destruct a. destruct (eq_rhs rh r) eqn:T.
-  + inv H. exists strict; auto.
-  + exploit IHeqs; eauto. intros [s IN]. exists s; auto.
+- destruct a. destruct (compat_rhs rh r) eqn:T.
+  + inv H. exists strict, r; auto using compat_rhs_sound.
+  + exploit IHeqs; eauto. intros (s & rh' & A & B). exists s, rh'; auto.
 Qed.
 
 Lemma find_valnum_num_charact:
@@ -238,22 +253,11 @@ Lemma find_rhs_sound:
   exists v, rhs_eval_to valu ge sp m rh v /\ Val.lessdef v rs#r.
 Proof.
   unfold find_rhs; intros. destruct (find_valnum_rhs' rh (num_eqs n)) as [vres|] eqn:E; try discriminate.
-  exploit find_valnum_rhs'_charact; eauto. intros [strict IN].
+  exploit find_valnum_rhs'_charact; eauto. intros (strict & rh' & IN & COMPAT).
   erewrite reg_valnum_sound by eauto.
   exploit num_holds_eq; eauto. intros EH. inv EH.
-- exists (valu vres); auto.
-- exists v; auto.
-Qed.
-
-Remark in_remove:
-  forall (A: Type) (eq: forall (x y: A), {x=y}+{x<>y}) x y l,
-  In y (List.remove eq x l) <-> x <> y /\ In y l.
-Proof.
-  induction l; simpl.
-  tauto.
-  destruct (eq x a).
-  subst a. rewrite IHl. tauto.
-  simpl. rewrite IHl. intuition congruence.
+- exists (valu vres); eauto using rhs_eval_to_compat, rhs_compat_sym.
+- exists v; eauto using rhs_eval_to_compat, rhs_compat_sym.
 Qed.
 
 Lemma forget_reg_charact:
@@ -264,7 +268,7 @@ Proof.
   unfold forget_reg; intros.
   destruct (PTree.get rd n.(num_reg)) as [vd|] eqn:GET.
 - rewrite PMap.gsspec in H0. destruct (peq v vd).
-  + subst v. rewrite in_remove in H0. intuition.
+  + subst v. apply List.in_remove in H0. tauto.
   + split; auto. exploit wf_num_val; eauto. congruence.
 - split; auto. exploit wf_num_val; eauto. congruence.
 Qed.
@@ -296,6 +300,7 @@ Qed.
 Lemma add_rhs_holds:
   forall valu1 ge sp rs m n rd rh rs',
   numbering_holds valu1 ge sp rs m n ->
+  rhs_valid valu1 ge sp rh ->
   rhs_eval_to valu1 ge sp m rh (rs'#rd) ->
   wf_rhs n.(num_next) rh ->
   (forall r, r <> rd -> rs'#r = rs#r) ->
@@ -305,10 +310,11 @@ Proof.
   destruct (find_valnum_rhs rh n.(num_eqs)) as [vres|] eqn:FIND.
 
 - (* A value number exists already *)
-  exploit find_valnum_rhs_charact; eauto. intros IN.
+  exploit find_valnum_rhs_charact; eauto. intros (rh' & IN & COMPAT).
   exploit wf_num_eqs; eauto with cse. intros [A B].
   exploit num_holds_eq; eauto. intros EH. inv EH.
-  assert (rs'#rd = valu1 vres) by (eapply rhs_eval_to_inj; eauto).
+  assert (rs'#rd = valu1 vres) by
+    (eapply rhs_eval_to_inj; eauto using rhs_eval_to_compat, rhs_compat_sym).
   exists valu1; constructor; simpl; intros.
 + constructor; simpl; intros.
   * eauto with cse.
@@ -319,7 +325,7 @@ Proof.
 + eauto with cse.
 + rewrite PTree.gsspec in H5. destruct (peq r rd).
   congruence.
-  rewrite H2 by auto. eauto with cse.
+  rewrite H3 by auto. eauto with cse.
 
 - (* Assigning a new value number *)
   set (valu2 := fun v => if peq v n.(num_next) then rs'#rd else valu1 v).
@@ -327,20 +333,21 @@ Proof.
   { red; intros. unfold valu2. apply peq_false. apply Plt_ne; auto. }
   exists valu2; constructor; simpl; intros.
 + constructor; simpl; intros.
-  * destruct H3. inv H3. simpl; split. extlia.
+  * destruct H4. inv H4. simpl; split. extlia.
     red; intros. apply Plt_trans_succ; eauto.
     apply wf_equation_incr with (num_next n). eauto with cse. extlia.
-  * rewrite PTree.gsspec in H3. destruct (peq r rd).
-    inv H3. extlia.
+  * rewrite PTree.gsspec in H4. destruct (peq r rd).
+    inv H4. extlia.
     apply Plt_trans_succ; eauto with cse.
   * apply update_reg_charact; eauto with cse.
-+ destruct H3. inv H3.
++ destruct H4. inv H4.
   constructor. unfold valu2 at 2; rewrite peq_true.
   eapply rhs_eval_to_exten; eauto.
+  eapply rhs_valid_exten; eauto.
   eapply equation_holds_exten; eauto with cse.
-+ rewrite PTree.gsspec in H3. unfold valu2. destruct (peq r rd).
-  inv H3. rewrite peq_true; auto.
-  rewrite peq_false. rewrite H2 by auto. eauto with cse.
++ rewrite PTree.gsspec in H4. unfold valu2. destruct (peq r rd).
+  inv H4. rewrite peq_true; auto.
+  rewrite peq_false. rewrite H3 by auto. eauto with cse.
   apply Plt_ne; eauto with cse.
 Qed.
 
@@ -373,22 +380,25 @@ Proof.
   exploit valnum_regs_holds; eauto.
   intros (valu2 & A & B & C & D & E).
   eapply add_rhs_holds; eauto.
++ constructor.
 + constructor. rewrite Regmap.gss. congruence.
 + intros. apply Regmap.gso; auto.
 Qed.
 
 Lemma add_load_holds:
-  forall valu1 ge sp rs m n addr (args: list reg) a chunk v dst,
-  numbering_holds valu1 ge sp rs m n ->
-  eval_addressing ge sp addr rs##args = Some a ->
-  Mem.loadv chunk m a = Some v ->
-  exists valu2, numbering_holds valu2 ge sp (rs#dst <- v) m (add_load n dst chunk addr args).
+  forall valu1 ge sp rs m n addr (args: list reg) ap b ofs chunk v dst bc,
+  numbering_holds valu1 ge (Vptr sp Ptrofs.zero) rs m n ->
+  eval_addressing ge (Vptr sp Ptrofs.zero) addr rs##args = Some (Vptr b ofs) ->
+  Mem.loadv chunk m (Vptr b ofs) = Some v ->
+  pmatch bc b ofs ap -> genv_match bc ge -> bc sp = BCstack ->
+  exists valu2, numbering_holds valu2 ge (Vptr sp Ptrofs.zero) (rs#dst <- v) m (add_load n dst chunk addr args ap).
 Proof.
   unfold add_load; intros.
   destruct (valnum_regs n args) as [n1 vl] eqn:VN.
   exploit valnum_regs_holds; eauto.
   intros (valu2 & A & B & C & D & E).
   eapply add_rhs_holds; eauto.
++ econstructor; eauto. rewrite <- B; auto. 
 + econstructor. rewrite <- B; eauto. rewrite Regmap.gss; auto.
 + intros. apply Regmap.gso; auto.
 Qed.
@@ -437,6 +447,7 @@ Lemma kill_equations_hold:
   numbering_holds valu ge sp rs m n ->
   (forall r v,
       pred r = false ->
+      rhs_valid valu ge sp r ->
       rhs_eval_to valu ge sp m r v ->
       rhs_eval_to valu ge sp m' r v) ->
   numbering_holds valu ge sp rs m' (kill_equations pred n).
@@ -455,8 +466,8 @@ Lemma kill_all_loads_hold:
   numbering_holds valu ge sp rs m' (kill_all_loads n).
 Proof.
   intros. eapply kill_equations_hold; eauto.
-  unfold filter_loads; intros. inv H1.
-  constructor. rewrite <- H2. apply op_depends_on_memory_correct; auto.
+  unfold filter_loads; intros. inv H2.
+  constructor. rewrite <- H3. apply op_depends_on_memory_correct; auto.
   discriminate.
 Qed.
 
@@ -473,19 +484,18 @@ Lemma kill_loads_after_store_holds:
                            (kill_loads_after_store approx n chunk addr args).
 Proof.
   intros. apply kill_equations_hold with m; auto.
-  intros. unfold filter_after_store in H6; inv H7.
-- constructor. rewrite <- H8. apply op_depends_on_memory_correct; auto.
-- destruct (regs_valnums n vl) as [rl|] eqn:RV; try discriminate.
-  econstructor; eauto. rewrite <- H9.
+  intros. unfold filter_after_store in H6; inv H8.
+- constructor. rewrite <- H9. apply op_depends_on_memory_correct; auto.
+- econstructor; eauto. rewrite <- H10.
   destruct a; simpl in H1; try discriminate.
-  destruct a0; simpl in H9; try discriminate.
+  destruct a0; simpl in H10; try discriminate.
   simpl.
   rewrite negb_false_iff in H6. unfold aaddressing in H6.
+  inv H7. rewrite H9 in H14; inv H14.
   eapply Mem.load_store_other. eauto.
-  eapply pdisjoint_sound. eauto.
+  eapply pdisjoint_sound_strong with (bc1 := bc0) (bc2 := bc); eauto.
   apply match_aptr_of_aval. eapply eval_static_addressing_sound; eauto.
-  erewrite <- regs_valnums_sound by eauto. eauto with va.
-  apply match_aptr_of_aval. eapply eval_static_addressing_sound; eauto with va.
+  eauto with va.
 Qed.
 
 Lemma store_normalized_range_sound:
@@ -507,15 +517,17 @@ Qed.
 
 Lemma add_store_result_hold:
   forall valu1 ge sp rs m' n addr args a chunk m src bc ae approx am,
-  numbering_holds valu1 ge sp rs m' n ->
-  eval_addressing ge sp addr rs##args = Some a ->
+  numbering_holds valu1 ge (Vptr sp Ptrofs.zero) rs m' n ->
+  eval_addressing ge (Vptr sp Ptrofs.zero) addr rs##args = Some a ->
   Mem.storev chunk m a rs#src = Some m' ->
+  genv_match bc ge ->
+  bc sp = BCstack ->
   ematch bc rs ae ->
   approx = VA.State ae am ->
-  exists valu2, numbering_holds valu2 ge sp rs m' (add_store_result approx n chunk addr args src).
+  exists valu2, numbering_holds valu2 ge (Vptr sp Ptrofs.zero) rs m' (add_store_result approx n chunk addr args src).
 Proof.
   unfold add_store_result; intros.
-  unfold avalue; rewrite H3.
+  unfold avalue; rewrite H5.
   destruct (vincl (AE.get src ae) (store_normalized_range chunk)) eqn:INCL.
 - destruct (valnum_reg n src) as [n1 vsrc] eqn:VR1.
   destruct (valnum_regs n1 args) as [n2 vargs] eqn:VR2.
@@ -523,46 +535,40 @@ Proof.
   exploit valnum_regs_holds; eauto. intros (valu3 & P & Q & R & S & T).
   exists valu3. constructor; simpl; intros.
 + constructor; simpl; intros; eauto with cse.
-  destruct H4; eauto with cse. subst e. split.
+  destruct H6; eauto with cse. subst e. split.
   eapply Pos.lt_le_trans; eauto.
   red; simpl; intros. auto.
-+ destruct H4; eauto with cse. subst eq. apply eq_holds_lessdef with (Val.load_result chunk rs#src).
-  apply load_eval_to with a. rewrite <- Q; auto.
-  destruct a; try discriminate. simpl. eapply Mem.load_store_same; eauto.
-  rewrite B. rewrite R by auto. apply store_normalized_range_sound with bc.
-  rewrite <- B. eapply vmatch_ge. apply vincl_ge; eauto. apply H2.
++ destruct H6; eauto with cse. subst eq. apply eq_holds_lessdef with (Val.load_result chunk rs#src).
+  * apply load_eval_to with a. rewrite <- Q; auto.
+    destruct a; try discriminate. simpl. eapply Mem.load_store_same; eauto.
+  * rewrite B. rewrite R by auto. apply store_normalized_range_sound with bc.
+    rewrite <- B. eapply vmatch_ge. apply vincl_ge; eauto. apply H4.
+  * destruct a; try discriminate. econstructor; eauto. rewrite <- Q. eassumption.
+    apply match_aptr_of_aval. eapply eval_static_addressing_sound; eauto with va.
 + eauto with cse.
-
 - exists valu1; auto.
 Qed.
 
 Lemma kill_loads_after_storebytes_holds:
-  forall valu ge sp rs m n dst b ofs bytes m' bc approx ae am sz,
+  forall valu ge sp rs m n dst b ofs bytes m' bc sz,
   numbering_holds valu ge (Vptr sp Ptrofs.zero) rs m n ->
   pmatch bc b ofs dst ->
   Mem.storebytes m b (Ptrofs.unsigned ofs) bytes = Some m' ->
   genv_match bc ge ->
   bc sp = BCstack ->
-  ematch bc rs ae ->
-  approx = VA.State ae am ->
   length bytes = Z.to_nat sz -> sz >= 0 ->
   numbering_holds valu ge (Vptr sp Ptrofs.zero) rs m'
-                           (kill_loads_after_storebytes approx n dst sz).
+                           (kill_loads_after_storebytes n dst sz).
 Proof.
   intros. apply kill_equations_hold with m; auto.
-  intros. unfold filter_after_store in H8; inv H9.
-- constructor. rewrite <- H10. apply op_depends_on_memory_correct; auto.
-- destruct (regs_valnums n vl) as [rl|] eqn:RV; try discriminate.
-  econstructor; eauto. rewrite <- H11.
-  destruct a; simpl in H10; try discriminate.
-  simpl.
-  rewrite negb_false_iff in H8.
+  intros. unfold filter_after_store in H6; inv H8.
+- constructor. rewrite <- H9. apply op_depends_on_memory_correct; auto.
+- inv H7. rewrite H9 in H15; inv H15.
+  econstructor; eauto. rewrite <- H10. simpl.
+  rewrite negb_false_iff in H6.
   eapply Mem.load_storebytes_other. eauto.
-  rewrite H6. rewrite Z2Nat.id by lia.
-  eapply pdisjoint_sound. eauto.
-  unfold aaddressing. apply match_aptr_of_aval. eapply eval_static_addressing_sound; eauto.
-  erewrite <- regs_valnums_sound by eauto. eauto with va.
-  auto.
+  rewrite H4. rewrite Z2Nat.id by lia.
+  eapply pdisjoint_sound_strong with (bc1 := bc0) (bc2 := bc); eauto.
 Qed.
 
 Lemma load_memcpy:
@@ -660,17 +666,20 @@ Proof with (try discriminate).
     unfold j, delta. eapply load_memcpy; eauto.
     apply Zmod_divide; auto. generalize (align_chunk_pos chunk); lia.
   }
+  rename a into ap.
+  assert (eval_addressing ge (Vptr sp Ptrofs.zero) (Ainstack (Ptrofs.repr j)) nil = Some (Vptr sp (Ptrofs.repr j))).
+  { rewrite eval_addressing_Ainstack. simpl. rewrite Ptrofs.add_zero_l. auto. }
   inv H2.
-+ inv H3. exploit eval_addressing_Ainstack_inv; eauto. intros [E1 E2].
++ inv H5. exploit eval_addressing_Ainstack_inv; eauto. intros [E1 E2].
   simpl in E2; rewrite Ptrofs.add_zero_l in E2. subst a.
-  apply eq_holds_strict. econstructor. rewrite eval_addressing_Ainstack.
-  simpl. rewrite Ptrofs.add_zero_l. eauto.
-  apply LD; auto.
-+ inv H4. exploit eval_addressing_Ainstack_inv; eauto. intros [E1 E2].
+  apply eq_holds_strict.
+  * econstructor; eauto.
+  * inv H7. econstructor; eauto with va.
++ inv H6. exploit eval_addressing_Ainstack_inv; eauto. intros [E1 E2].
   simpl in E2; rewrite Ptrofs.add_zero_l in E2. subst a.
   apply eq_holds_lessdef with v; auto.
-  econstructor. rewrite eval_addressing_Ainstack. simpl. rewrite Ptrofs.add_zero_l. eauto.
-  apply LD; auto.
+  * econstructor; eauto.
+  * inv H8. econstructor; eauto with va.
 Qed.
 
 Lemma add_memcpy_eqs_charact:
@@ -810,13 +819,11 @@ Proof.
   destruct (f (fun v : valnum => find_valnum_num v (num_eqs n)) op args)
            as [[op1 args1] | ] eqn:?; try discriminate.
   assert (exists r': val, sem op1 (map valu args1) = Some r' /\ Val.lessdef r r').
-  { exploit f_sound.
+  { exploit f_sound; eauto.
     simpl; intros.
     exploit num_holds_eq; eauto.
     eapply find_valnum_num_charact; eauto with cse.
-    eapply H1.
-    intros EH; inv EH; auto. eexact H3. eexact Heqo. eexact H0.
-    intros. eauto.
+    intros EH; inv EH; auto.
   }
   destruct (reduce_rec A f n niter op1 args1) as [[op2 rl2] | ] eqn:?.
   destruct H1. destruct H1.
@@ -1102,7 +1109,7 @@ Proof.
   destruct (valnum_regs approx!!pc args) as [n1 vl] eqn:?.
   destruct SAT as [valu1 NH1].
   exploit valnum_regs_holds; eauto. intros (valu2 & NH2 & EQ & AG & P & Q).
-  destruct (find_rhs n1 (Load chunk addr vl)) as [r|] eqn:?.
+  destruct (find_rhs n1 (Load chunk addr vl Ptop)) as [r|] eqn:?.
 + (* replaced by move *)
   exploit find_rhs_sound; eauto. intros (v' & EV & LD).
   assert (v' = v) by (inv EV; congruence). subst v'.
@@ -1111,7 +1118,10 @@ Proof.
   econstructor; eauto.
   eapply analysis_correct_1; eauto. simpl; auto.
   unfold transfer; rewrite H.
+  destruct a; try discriminate. InvSoundState.
   eapply add_load_holds; eauto.
+  unfold aaddressing, vanalyze. rewrite AN. apply match_aptr_of_aval.
+  eapply eval_static_addressing_sound; eauto with va.
   apply set_reg_lessdef; auto. eapply Val.lessdef_trans; eauto.
 + (* load is preserved, but addressing is possibly simplified *)
   destruct (reduce addressing combine_addr n1 addr args vl) as [addr' args'] eqn:?.
@@ -1129,7 +1139,10 @@ Proof.
   econstructor; eauto.
   eapply analysis_correct_1; eauto. simpl; auto.
   unfold transfer; rewrite H.
+  destruct a; try discriminate. InvSoundState.
   eapply add_load_holds; eauto.
+  unfold aaddressing, vanalyze. rewrite AN. apply match_aptr_of_aval.
+  eapply eval_static_addressing_sound; eauto with va.
   apply set_reg_lessdef; auto.
 
 - (* Istore *)
